Verified.lean
@@ -1,5 +1,10 @@
 -- This module serves as the root of the `Verified` library.
 -- Import modules here that should be built as part of the library.
-import Verified.Imp.Syntax
-import Verified.Imp.Semantics
-import Verified.Imp.Properties
+import Verified.VAE.Syntax
+import Verified.VAE.BigStep
+import Verified.IMP.Syntax
+import Verified.IMP.BigStep
+import Verified.IMP.BigStep.Properties
+import Verified.VAE.SmallStep
+import Verified.VAE.SmallStep.Properties
+import Verified.IMP.SmallStep
