Verified/VAE/BigStep.lean
@@ -1,0 +1,18 @@
+import Verified.VAE.Syntax
+
+namespace VAE
+
+inductive Eval : Env -> Expr -> Int -> Prop where
+  | num n : Eval env (.num n) n
+  | add :
+    Eval env e1 n1 -> Eval env e2 n2 ->
+    Eval env (.add e1 e2) (n1 + n2)
+  | mul :
+    Eval env e1 n1 -> Eval env e2 n2 ->
+    Eval env (.mul e1 e2) (n1 * n2)
+  | val :
+    Eval env e1 n1 -> Eval (Env.update env x n1) e2 n2 ->
+    Eval env (.val x e1 e2) n2
+  | id : env x = some n -> Eval env (.id x) n
+
+end VAE
