Verified/VAE/Syntax.lean
@@ -1,0 +1,16 @@
+namespace VAE
+
+inductive Expr where
+  | num (n : Int)
+  | add (e1 e2 : Expr)
+  | mul (e1 e2 : Expr)
+  | val (x : String) (e1 : Expr) (e2 : Expr)
+  | id (x : String)
+
+abbrev Env := String -> Option Int
+
+-- helper: update the environment
+def Env.update (env : Env) (x : String) (v : Int) : Env :=
+  fun y => if y == x then some v else env y
+
+end VAE
